.

theories/Prelude/PreludeMath.v
@@ -1,17 +1,166 @@
+Require Import Coq.Classes.RelationClasses.
+Require Import Coq.Lists.List.
+Require Import Coq.Program.Basics.
+Require Import Coq.Relations.Relation_Definitions.
+Require Import Coq.Relations.Relation_Operators.
+Require Import Coq.Setoids.Setoid.
 Require Import DschingisKhan.Prelude.PreludeInit.
 
 Module MathPrelude.
 
-  Polymorphic Class isCountable (X : Hask.t) : Type :=
-    { enum (n : nat) : X
-    ; enumeratable (x : X) : exists n : nat, enum n = x
+  Local Open Scope program_scope.
+
+  (** "0. Utilities" *)
+
+  Class isUnaryOperationCompatibleWithSetoid {dom : Hask.t} {cod : Hask.t} {dom_isSetoid : isSetoid dom} {cod_isSetoid : isSetoid cod} (f : dom -> cod) : Prop :=
+    unary_operation_preserves_eqProp (lhs : dom) (rhs : dom) (H_EQ : lhs == rhs) : f lhs == f rhs
+  .
+
+  Class isBinaryOperationCompatibleWithSetoid {dom1 : Hask.t} {dom2 : Hask.t} {cod : Hask.t} {dom1_isSetoid : isSetoid dom1} {dom2_isSetoid : isSetoid dom2} {cod_isSetoid : isSetoid cod} (f : dom1 -> dom2 -> cod) : Prop :=
+    binary_operation_preserves_eqProp (lhs1 : dom1) (rhs1 : dom1) (lhs2 : dom2) (rhs2 : dom2) (H_EQ1 : lhs1 == rhs1) (H_EQ2 : lhs2 == rhs2) : f lhs1 lhs2 == f rhs1 rhs2
+  .
+
+  Global Add Parametric Morphism {dom : Hask.t} {cod : Hask.t} {dom_isSetoid : isSetoid dom} {cod_isSetoid : isSetoid cod} (f : dom -> cod) {f_isCompatible : isUnaryOperationCompatibleWithSetoid f} :
+    f with signature (eqProp ==> eqProp)
+    as unary_operation_lifts_eqProp.
+  Proof. ii; apply f_isCompatible; eauto. Qed.
+
+  Global Add Parametric Morphism {dom1 : Hask.t} {dom2 : Hask.t} {cod : Hask.t} {dom1_isSetoid : isSetoid dom1} {dom2_isSetoid : isSetoid dom2} {cod_isSetoid : isSetoid cod} (f : dom1 -> dom2 -> cod) {f_isCompatible : isBinaryOperationCompatibleWithSetoid f} :
+    f with signature (eqProp ==> eqProp ==> eqProp)
+    as binary_operation_lifts_eqProp.
+  Proof. ii; apply f_isCompatible; eauto. Qed.
+
+  Section STATEMENTS_FOR_OPERATION_PROPERTIES.
+
+  Context {A : Hask.t} {requiresSetoid : isSetoid A}.
+
+  Class isAssociativeBinaryOperation (bin_op : A -> A -> A) : Prop :=
+    bin_op_assoc (x : A) (y : A) (z : A) : bin_op x (bin_op y z) == bin_op (bin_op x y) z
+  .
+
+  Class isCommutativeBinaryOperation (bin_op : A -> A -> A) : Prop :=
+    bin_op_comm (x : A) (y : A) : bin_op x y == bin_op y x
+  .
+
+  Class isIdempotentBinaryOperation (bin_op : A -> A -> A) : Prop :=
+    idemponence (x : A) : bin_op x x == x
+  .
+
+  Class isDistributiveOver (bin_op1 : A -> A -> A) (bin_op2 : A -> A -> A) : Prop :=
+    { left_distr (x : A) (y : A) (z : A) : bin_op1 x (bin_op2 y z) == bin_op2 (bin_op1 x y) (bin_op1 x z)
+    ; right_distr (x : A) (y : A) (z : A) : bin_op1 (bin_op2 y z) x == bin_op2 (bin_op1 y x) (bin_op1 z x)
+    }
+  .
+
+  Class isIdentity (e : A) (bin_op : A -> A -> A) : Prop :=
+    { left_id (x : A) : bin_op e x == x
+    ; right_id (x : A) : bin_op x e == x
+    }
+  .
+
+  Class isInverseOperation (inv : A -> A) (bin_op : A -> A -> A) : Prop :=
+    { left_inv (x : A) : bin_op (inv x) x == x
+    ; right_inv (x : A) : bin_op x (inv x) == x
+    }
+  .
+
+  Class linkedByAbsorptionLaw (bin_op1 : A -> A -> A) (bin_op2 : A -> A -> A) : Prop :=
+    { abosortion_left (x : A) (y : A) : bin_op1 x (bin_op2 x y) == x
+    ; abosortion_right (x : A) (y : A) : bin_op2 x (bin_op1 x y) == x
+    }
+  .
+
+  End STATEMENTS_FOR_OPERATION_PROPERTIES.
+
+  Global Infix " `distributesOver` " := isDistributiveOver (at level 70, no associativity) : type_scope.
+  Global Infix " `isIdentityOf` " := isIdentity (at level 70, no associativity) : type_scope.
+  Global Infix " `isInverseOpFor` " := isInverseOperation (at level 70, no associativity) : type_scope.
+
+  Class isCountable (A : Hask.t) : Type :=
+    { enum (n : nat) : A
+    ; enumeratable (x : A) : exists n : nat, enum n = x
+    }
+  .
+
+  (** "1. CPO and CoLa" *)
+
+  Definition isUpperBound {D : Hask.t} {requiresPoset : isPoset D} (upper_bound_of_X : D) (X : ensemble D) : Prop :=
+    forall x : D, member x X -> x =< upper_bound_of_X
+  .
+
+  Definition isSupremumOf {D : Hask.t} {requiresPoset : isPoset D} (sup_X : D) (X : ensemble D) : Prop :=
+    forall upper_bound_of_X : D, isUpperBound upper_bound_of_X X <-> sup_X =< upper_bound_of_X
+  .
+
+  Class isCoLa (D : Hask.t) {requiresPoset : isPoset D} : Type :=
+    CoLa_isCompleteLattice (X : ensemble D) : {sup_X : D | isSupremumOf sup_X X}
+  .
+
+  Definition isDirectedSubset {D : Hask.t} {requiresPoset : isPoset D} (X : ensemble D) : Prop :=
+    forall x1 : D, member x1 X ->
+    forall x2 : D, member x2 X ->
+    exists x3 : D, member x3 X /\
+    <{ DIRECT : x1 =< x3 /\ x2 =< x3 }>
+  .
+
+  Class isCPO (D : Hask.t) {requiresPoset : isPoset D} : Type :=
+    CPO_isCompletePartialOrder (X : ensemble D) (X_isDirected : isDirectedSubset X) : {sup_X : D | isSupremumOf sup_X X}
+  .
+
+  (** "2. Topology" *)
+
+  Class isTopologicalSpace (A : Hask.t) : Type :=
+    { isOpen (X : ensemble A) : Prop
+    ; fullOpen
+      : isOpen full
+    ; unionsOpen
+      (Xs : ensemble (ensemble A))
+      (every_member_of_Xs_isOpen : forall X : ensemble A, member X Xs -> isOpen X)
+      : isOpen (unions Xs)
+    ; intersectionOpen
+      (X1 : ensemble A)
+      (X2 : ensemble A)
+      (X1_isOpen : isOpen X1)
+      (X2_isOpen : isOpen X2)
+      : isOpen (intersection X1 X2)
+    ; isOpen_eqProp_isOpen
+      (X1 : ensemble A)
+      (X2 : ensemble A)
+      (X1_isOpen : isOpen X1)
+      (X1_eq_X2 : X1 == X2)
+      : isOpen X2
+    }
+  .
+
+  (** "3. Semigroup, Monoid and Group" *)
+
+  Class isSemigroup (S : Hask.t) {requiresSetoid : isSetoid S} : Type :=
+    { plu : S -> S -> S
+    ; plu_lifts_eqProp :> isBinaryOperationCompatibleWithSetoid plu
+    ; plu_assoc :> isAssociativeBinaryOperation plu
+    }
+  .
+
+  Class isMonoid (M : Hask.t) {requiresSetoid : isSetoid M} : Type :=
+    { zer : M
+    ; Monoid_requiresSemigroup :> isSemigroup M
+    ; zer_id_plu :> zer `isIdentityOf` plu
+    }
+  .
+
+  Class isGroup (G : Hask.t) {requiresSetoid : isSetoid G} : Type :=
+    { neg : G -> G
+    ; Group_requiresMonoid :> isMonoid G
+    ; neg_inv_plu :> neg `isInverseOpFor` plu
+    }
+  .
+
+  Class isAbelianGroup (G : Hask.t) {requiresSetoid : isSetoid G} : Type :=
+    { AbelianGroup_requiresGroup :> isGroup G
+    ; plu_comm :> isCommutativeBinaryOperation plu
     }
   .
 
 End MathPrelude.
 
 Export MathPrelude.
-
-Module UndergraduateAlgebra.
-
-End UndergraduateAlgebra.
